CircuitSATEncoding.dfy
@@ -1,305 +1,305 @@
-include "Certificate.dfy"
-include "Circuit.dfy"
-include "CKTInput.dfy"
-function circuitToInput (c:circuit) : seq<string>
-    requires isCircuitGood(c)
-{
-    circuitToInput'(c,0)
-}
-function circuitCellToString (e:circuitCell) : string
-{
-    match e 
-        case AND => "AND"
-        case OR => "OR"
-        case NOT => "NOT"
-        case VARIABLE(x) => "VARIABLE"
-        case POZ(nr) =>
-            natToString(nr)
-}
-lemma stringToCircuitCellToStringIsTheSame (s:string,pos:nat)
-    requires !(s in ["AND","OR","NOT","VARIABLE"]) ==> isStringAValidNumber(s)
-    ensures circuitCellToString(stringToCircuitCell(s,pos))==s
-{
-    var c:=stringToCircuitCell(s,pos);
-    if isStringAValidNumber(s)
-    {
-        assert c==POZ(stringToNat(s));
-        assert isCircuitCellAPoz(c);
-        var s2:=circuitCellToString(c);
-        assert s2==natToString(stringToNat(s));
-        stringToNatThenNatToStringIdem(s);
-        assert s2==s;
-    }
-}
-function circuitToInput' (c:circuit,pos:nat) :seq<string>
-    requires pos<=|c|
-    requires isCircuitGood(c)
-    ensures |circuitToInput'(c,|c|)|==0
-    ensures pos<|c| ==> |circuitToInput'(c,pos)|==|circuitToInput'(c,pos+1)|+1
-    decreases |c|-pos
-{
-    if pos==|c| then 
-    []
-    else 
-        [circuitCellToString(c[pos])]+circuitToInput'(c,pos+1)
-}
-
-lemma sameCircuitToInputLength(c: circuit, poz: nat)
-    requires isCircuitGood(c)
-    requires poz <= |c|
-    ensures |circuitToInput'(c, poz)| == |c| - poz
-    decreases |c| - poz
-{
-    if poz == |c| {
-    } else {
-        sameCircuitToInputLength(c, poz + 1);
-    }
-}
-
-lemma sameFullCircuitToInputLength(c: circuit)
-    requires isCircuitGood(c)
-    ensures |circuitToInput(c)| == |c|
-{
-    sameCircuitToInputLength(c, 0);
-}
-
-function stringToCircuitCell (s:string,nr:nat):circuitCell
-    requires !(s in ["AND","OR","NOT","VARIABLE"]) ==> isStringAValidNumber(s) 
-{
-    match s
-        case "AND" => AND
-        case "OR" => OR
-        case "NOT" => NOT
-        case "VARIABLE" => VARIABLE("VARIABLE "+natToString(nr))
-        case _ => POZ(stringToNat(s))
-}
-
-function inputToCircuit (input:seq<string>) : circuit
-    requires isInputGoodForCKT(input)
-
- {
-     inputToCircuit'(input,0)
- }
-function inputToCircuit' (input:seq<string>,pos:nat) : circuit
-    requires pos<=|input|
-    requires isInputGoodForCKT(input)
-    decreases |input|-pos
-    ensures |inputToCircuit'(input,|input|)|==0
-    ensures pos<|input| ==> |inputToCircuit'(input,pos)|==|inputToCircuit'(input,pos+1)|+1
-{
-    if pos==|input| then []
-    else
-        [stringToCircuitCell(input[pos],pos)]+inputToCircuit'(input,pos+1)
-}
-lemma sameInputToCircuitLength(input:seq<string>, poz: nat)
-    requires isInputGoodForCKT(input)
-    requires poz <= |input|
-    ensures |inputToCircuit'(input, poz)| == |input| - poz
-    decreases |input| - poz
-{
-    if poz == |input| {
-    } else {
-        sameInputToCircuitLength(input, poz + 1);
-    }
-}
-
-lemma sameFullInputToCircuitLength(input:seq<string>)
-    requires isInputGoodForCKT(input)
-    ensures |inputToCircuit(input)| == |input|
-{
-    sameInputToCircuitLength(input, 0);
-}
-
-lemma InputToCircuit_IsGood(input: seq<string>)
-    requires isInputGoodForCKT(input)
-    ensures isCircuitGood(inputToCircuit(input))
-{
-    var c := inputToCircuit(input);
-    for pos:=0 to |c|
-        invariant forall poz:nat::0<=poz<pos ==>  isCircuitGood'(c[poz], poz) 
-    {
-            sameFullInputToCircuitLength(input);
-            Lemma_NthElement_Bridge(input, 0, pos); 
-            assert c[pos] == stringToCircuitCell(input[pos], pos);
-            if (isStringAValidNumber(input[pos]))
-            {
-                assert isStringGoodForCKT(input[pos],pos);
-                assert stringToNat(input[pos])<pos;
-                assert isCircuitCellAPoz(c[pos]);
-                assert match c[pos]
-                        case POZ(nr) => nr== stringToNat(input[pos]);
-                assert  match c[pos]
-                        case POZ(nr) => nr<pos;
-            }
-    }
-    
-}
-
-lemma Lemma_NthElement_Bridge(input: seq<string>, current: nat, target: nat)
-    requires isInputGoodForCKT(input)
-    requires current <= target < |input|
-    ensures var c_sub := inputToCircuit'(input, current);
-            target - current < |c_sub| &&
-            c_sub[target - current] == stringToCircuitCell(input[target],target)
-    decreases target - current
-{
-    if current == target {
-    } else {
-        Lemma_NthElement_Bridge(input, current + 1, target);
-    }
-}
-lemma NthElementBridge(c:circuit, current:nat, target:nat)
-    requires isCircuitGood(c)
-    requires current <= target <|c|
-    ensures var i_sub := circuitToInput'(c,current);
-            target-current<|i_sub| &&
-            (
-                i_sub[target-current] == circuitCellToString(c[target])
-            )
-    decreases target - current
-{
- if current == target {
-    } else {
-        NthElementBridge(c, current + 1, target);
-    }
-}
-lemma InputToCircuitSymmetry(input: seq<string>)
-    requires isInputGoodForCKT(input)
-    ensures isCircuitGood(inputToCircuit(input)) 
-    ensures circuitToInput(inputToCircuit(input)) == input 
-{
-    sameFullInputToCircuitLength(input);
-    assert |inputToCircuit(input)|==|input|;
-    FullInputToCircuitSymmetry(input, 0);
-}
-lemma FullInputToCircuitSymmetry(input: seq<string>, k: nat)
-    requires isInputGoodForCKT(input) && k <= |input|
-    requires |inputToCircuit(input)| == |input|
-    ensures isCircuitGood(inputToCircuit(input))
-    ensures var c := inputToCircuit(input);
-            circuitToInput'(c, k) == input[k..]
-    decreases |input| - k
-{
-    InputToCircuit_IsGood(input);
-    var c := inputToCircuit(input);
-    
-    if k == |input| {
-    } else {
-
-        Lemma_NthElement_Bridge(input, 0, k); 
-        stringToCircuitCellToStringIsTheSame(input[k],k);
-        assert c[k] == stringToCircuitCell(input[k], k);
-        assert circuitCellToString(c[k]) == input[k]; 
-        
-    }
-}
-lemma Lemma_NumberInputImpliesValidPos(input: seq<string>, k: nat)
-    requires k < |input|
-    requires isInputCKT'(input, k)
-    requires isStringAValidNumber(input[k])
-    ensures isStringAValidPos(input, k)
-{
-    assert match input[k]
-        case "AND" => false
-        case "OR" => false
-        case "NOT" => false
-        case "VARIABLE" => false
-        case _ => true;
-}
-
-// 
-// lemma validCircuitGivesCKTInput(c:circuit) 
-//     requires isCircuitValid(c)
-//     ensures isCircuitGood(c) && isInputCKT(circuitToInput(c))
+// include "Certificate.dfy"
+// include "Circuit.dfy"
+// include "CKTInput.dfy"
+// function circuitToInput (c:circuit) : seq<string>
+//     requires isCircuitGood(c)
 // {
-//     aValidCircuitIsGood(c);
-//     var input := circuitToInput(c);
-//     sameFullCircuitToInputLength(c);
-//     assert |c| == |input|;
-    
-//     for i := 0 to |input|
-//         invariant forall poz:nat :: poz < i ==> isInputCKT'(input, poz)
+//     circuitToInput'(c,0)
+// }
+// function circuitCellToString (e:circuitCell) : string
+// {
+//     match e 
+//         case AND => "AND"
+//         case OR => "OR"
+//         case NOT => "NOT"
+//         case VARIABLE(x) => "VARIABLE"
+//         case POZ(nr) =>
+//             natToString(nr)
+// }
+// lemma stringToCircuitCellToStringIsTheSame (s:string,pos:nat)
+//     requires !(s in ["AND","OR","NOT","VARIABLE"]) ==> isStringAValidNumber(s)
+//     ensures circuitCellToString(stringToCircuitCell(s,pos))==s
+// {
+//     var c:=stringToCircuitCell(s,pos);
+//     if isStringAValidNumber(s)
 //     {
-//         NthElementBridge(c, 0, i);
-//         assert isCircuitValid'(c, i);
-        
-//         match c[i]
-//             case POZ(n) => {
-//                 assert n < i;
-//                 assert !isCircuitCellAPoz(c[n]);
-//                 NthElementBridge(c, 0, n); 
-//                 assert input[n] == circuitCellToString(c[n]);
-//                 assert !isStringAValidNumber(input[n]); 
-//                 natToStringThenStringToNatIdem(n);
-//                 assert isStringAValidPos(input, i);
-//                 assert isInputCKT'(input, i);
-//             }
-//             case AND => {
-//                 assert i >= 2;  
-//                 assert isCircuitCellAPoz(c[i-1]);
-//                 assert isCircuitCellAPoz(c[i-2]);
-                
-//                 NthElementBridge(c, 0, i-1);
-//                 NthElementBridge(c, 0, i-2);
-                
-//                 var s1 := input[i-1];
-//                 var s2 := input[i-2];
-                
-//                 assert match c[i-1] case POZ(_) => isStringAValidNumber(s1);
-//                 assert match c[i-2] case POZ(_) => isStringAValidNumber(s2);
-                
-//                 assert isStringAValidNumber(s1);
-//                 assert isStringAValidNumber(s2);
-//                 assert isInputCKT'(input, i);
-//             }
-//             case OR => {
-//                 assert i >= 2;
-//                 assert isCircuitCellAPoz(c[i-1]);
-//                 assert isCircuitCellAPoz(c[i-2]);
-                
-//                 NthElementBridge(c, 0, i-1);
-//                 NthElementBridge(c, 0, i-2);
-                
-//                 var s1 := input[i-1];
-//                 var s2 := input[i-2];
-                
-//                 assert match c[i-1] case POZ(_) => isStringAValidNumber(s1);
-//                 assert match c[i-2] case POZ(_) => isStringAValidNumber(s2);
-                
-//                 assert isStringAValidNumber(s1);
-//                 assert isStringAValidNumber(s2);
-//                 assert isInputCKT'(input, i);
-//             }
-//             case NOT => {
-//                 assert i >= 1;
-//                 assert isCircuitCellAPoz(c[i-1]);
-                
-//                 NthElementBridge(c, 0, i-1);
-//                 var s1 := input[i-1];
-                
-//                 assert match c[i-1] case POZ(_) => isStringAValidNumber(s1);
-//                 assert isStringAValidNumber(s1);
-                
-//                 assert isInputCKT'(input, i);
-//             }
-//             case VARIABLE(X) => {
-//                 assert isInputCKT'(input, i);
-//             }
+//         assert c==POZ(stringToNat(s));
+//         assert isCircuitCellAPoz(c);
+//         var s2:=circuitCellToString(c);
+//         assert s2==natToString(stringToNat(s));
+//         stringToNatThenNatToStringIdem(s);
+//         assert s2==s;
+//     }
+// }
+// function circuitToInput' (c:circuit,pos:nat) :seq<string>
+//     requires pos<=|c|
+//     requires isCircuitGood(c)
+//     ensures |circuitToInput'(c,|c|)|==0
+//     ensures pos<|c| ==> |circuitToInput'(c,pos)|==|circuitToInput'(c,pos+1)|+1
+//     decreases |c|-pos
+// {
+//     if pos==|c| then 
+//     []
+//     else 
+//         [circuitCellToString(c[pos])]+circuitToInput'(c,pos+1)
+// }
+
+// lemma sameCircuitToInputLength(c: circuit, poz: nat)
+//     requires isCircuitGood(c)
+//     requires poz <= |c|
+//     ensures |circuitToInput'(c, poz)| == |c| - poz
+//     decreases |c| - poz
+// {
+//     if poz == |c| {
+//     } else {
+//         sameCircuitToInputLength(c, poz + 1);
 //     }
 // }
 
-lemma PozCellGivesValidNumber(c: circuit, pos: nat, input: seq<string>)
-    requires isCircuitValid(c)
-    requires pos < |c|
-    requires isCircuitCellAPoz(c[pos])
-    requires isCircuitGood(c)
-    requires input == circuitToInput(c)
-    requires |input| == |c|
-    ensures isStringAValidNumber(input[pos])
-{
-    NthElementBridge(c, 0, pos);
-    assert input[pos] == circuitCellToString(c[pos]);
-}
+// lemma sameFullCircuitToInputLength(c: circuit)
+//     requires isCircuitGood(c)
+//     ensures |circuitToInput(c)| == |c|
+// {
+//     sameCircuitToInputLength(c, 0);
+// }
+
+// function stringToCircuitCell (s:string,nr:nat):circuitCell
+//     requires !(s in ["AND","OR","NOT","VARIABLE"]) ==> isStringAValidNumber(s) 
+// {
+//     match s
+//         case "AND" => AND
+//         case "OR" => OR
+//         case "NOT" => NOT
+//         case "VARIABLE" => VARIABLE("VARIABLE "+natToString(nr))
+//         case _ => POZ(stringToNat(s))
+// }
+
+// function inputToCircuit (input:seq<string>) : circuit
+//     requires isInputGoodForCKT(input)
+
+//  {
+//      inputToCircuit'(input,0)
+//  }
+// function inputToCircuit' (input:seq<string>,pos:nat) : circuit
+//     requires pos<=|input|
+//     requires isInputGoodForCKT(input)
+//     decreases |input|-pos
+//     ensures |inputToCircuit'(input,|input|)|==0
+//     ensures pos<|input| ==> |inputToCircuit'(input,pos)|==|inputToCircuit'(input,pos+1)|+1
+// {
+//     if pos==|input| then []
+//     else
+//         [stringToCircuitCell(input[pos],pos)]+inputToCircuit'(input,pos+1)
+// }
+// lemma sameInputToCircuitLength(input:seq<string>, poz: nat)
+//     requires isInputGoodForCKT(input)
+//     requires poz <= |input|
+//     ensures |inputToCircuit'(input, poz)| == |input| - poz
+//     decreases |input| - poz
+// {
+//     if poz == |input| {
+//     } else {
+//         sameInputToCircuitLength(input, poz + 1);
+//     }
+// }
+
+// lemma sameFullInputToCircuitLength(input:seq<string>)
+//     requires isInputGoodForCKT(input)
+//     ensures |inputToCircuit(input)| == |input|
+// {
+//     sameInputToCircuitLength(input, 0);
+// }
+
+// lemma InputToCircuit_IsGood(input: seq<string>)
+//     requires isInputGoodForCKT(input)
+//     ensures isCircuitGood(inputToCircuit(input))
+// {
+//     var c := inputToCircuit(input);
+//     for pos:=0 to |c|
+//         invariant forall poz:nat::0<=poz<pos ==>  isCircuitGood'(c[poz], poz) 
+//     {
+//             sameFullInputToCircuitLength(input);
+//             Lemma_NthElement_Bridge(input, 0, pos); 
+//             assert c[pos] == stringToCircuitCell(input[pos], pos);
+//             if (isStringAValidNumber(input[pos]))
+//             {
+//                 assert isStringGoodForCKT(input[pos],pos);
+//                 assert stringToNat(input[pos])<pos;
+//                 assert isCircuitCellAPoz(c[pos]);
+//                 assert match c[pos]
+//                         case POZ(nr) => nr== stringToNat(input[pos]);
+//                 assert  match c[pos]
+//                         case POZ(nr) => nr<pos;
+//             }
+//     }
+    
+// }
+
+// lemma Lemma_NthElement_Bridge(input: seq<string>, current: nat, target: nat)
+//     requires isInputGoodForCKT(input)
+//     requires current <= target < |input|
+//     ensures var c_sub := inputToCircuit'(input, current);
+//             target - current < |c_sub| &&
+//             c_sub[target - current] == stringToCircuitCell(input[target],target)
+//     decreases target - current
+// {
+//     if current == target {
+//     } else {
+//         Lemma_NthElement_Bridge(input, current + 1, target);
+//     }
+// }
+// lemma NthElementBridge(c:circuit, current:nat, target:nat)
+//     requires isCircuitGood(c)
+//     requires current <= target <|c|
+//     ensures var i_sub := circuitToInput'(c,current);
+//             target-current<|i_sub| &&
+//             (
+//                 i_sub[target-current] == circuitCellToString(c[target])
+//             )
+//     decreases target - current
+// {
+//  if current == target {
+//     } else {
+//         NthElementBridge(c, current + 1, target);
+//     }
+// }
+// lemma InputToCircuitSymmetry(input: seq<string>)
+//     requires isInputGoodForCKT(input)
+//     ensures isCircuitGood(inputToCircuit(input)) 
+//     ensures circuitToInput(inputToCircuit(input)) == input 
+// {
+//     sameFullInputToCircuitLength(input);
+//     assert |inputToCircuit(input)|==|input|;
+//     FullInputToCircuitSymmetry(input, 0);
+// }
+// lemma FullInputToCircuitSymmetry(input: seq<string>, k: nat)
+//     requires isInputGoodForCKT(input) && k <= |input|
+//     requires |inputToCircuit(input)| == |input|
+//     ensures isCircuitGood(inputToCircuit(input))
+//     ensures var c := inputToCircuit(input);
+//             circuitToInput'(c, k) == input[k..]
+//     decreases |input| - k
+// {
+//     InputToCircuit_IsGood(input);
+//     var c := inputToCircuit(input);
+    
+//     if k == |input| {
+//     } else {
+
+//         Lemma_NthElement_Bridge(input, 0, k); 
+//         stringToCircuitCellToStringIsTheSame(input[k],k);
+//         assert c[k] == stringToCircuitCell(input[k], k);
+//         assert circuitCellToString(c[k]) == input[k]; 
+        
+//     }
+// }
+// lemma Lemma_NumberInputImpliesValidPos(input: seq<string>, k: nat)
+//     requires k < |input|
+//     requires isInputCKT'(input, k)
+//     requires isStringAValidNumber(input[k])
+//     ensures isStringAValidPos(input, k)
+// {
+//     assert match input[k]
+//         case "AND" => false
+//         case "OR" => false
+//         case "NOT" => false
+//         case "VARIABLE" => false
+//         case _ => true;
+// }
+
+// // 
+// // lemma validCircuitGivesCKTInput(c:circuit) 
+// //     requires isCircuitValid(c)
+// //     ensures isCircuitGood(c) && isInputCKT(circuitToInput(c))
+// // {
+// //     aValidCircuitIsGood(c);
+// //     var input := circuitToInput(c);
+// //     sameFullCircuitToInputLength(c);
+// //     assert |c| == |input|;
+    
+// //     for i := 0 to |input|
+// //         invariant forall poz:nat :: poz < i ==> isInputCKT'(input, poz)
+// //     {
+// //         NthElementBridge(c, 0, i);
+// //         assert isCircuitValid'(c, i);
+        
+// //         match c[i]
+// //             case POZ(n) => {
+// //                 assert n < i;
+// //                 assert !isCircuitCellAPoz(c[n]);
+// //                 NthElementBridge(c, 0, n); 
+// //                 assert input[n] == circuitCellToString(c[n]);
+// //                 assert !isStringAValidNumber(input[n]); 
+// //                 natToStringThenStringToNatIdem(n);
+// //                 assert isStringAValidPos(input, i);
+// //                 assert isInputCKT'(input, i);
+// //             }
+// //             case AND => {
+// //                 assert i >= 2;  
+// //                 assert isCircuitCellAPoz(c[i-1]);
+// //                 assert isCircuitCellAPoz(c[i-2]);
+                
+// //                 NthElementBridge(c, 0, i-1);
+// //                 NthElementBridge(c, 0, i-2);
+                
+// //                 var s1 := input[i-1];
+// //                 var s2 := input[i-2];
+                
+// //                 assert match c[i-1] case POZ(_) => isStringAValidNumber(s1);
+// //                 assert match c[i-2] case POZ(_) => isStringAValidNumber(s2);
+                
+// //                 assert isStringAValidNumber(s1);
+// //                 assert isStringAValidNumber(s2);
+// //                 assert isInputCKT'(input, i);
+// //             }
+// //             case OR => {
+// //                 assert i >= 2;
+// //                 assert isCircuitCellAPoz(c[i-1]);
+// //                 assert isCircuitCellAPoz(c[i-2]);
+                
+// //                 NthElementBridge(c, 0, i-1);
+// //                 NthElementBridge(c, 0, i-2);
+                
+// //                 var s1 := input[i-1];
+// //                 var s2 := input[i-2];
+                
+// //                 assert match c[i-1] case POZ(_) => isStringAValidNumber(s1);
+// //                 assert match c[i-2] case POZ(_) => isStringAValidNumber(s2);
+                
+// //                 assert isStringAValidNumber(s1);
+// //                 assert isStringAValidNumber(s2);
+// //                 assert isInputCKT'(input, i);
+// //             }
+// //             case NOT => {
+// //                 assert i >= 1;
+// //                 assert isCircuitCellAPoz(c[i-1]);
+                
+// //                 NthElementBridge(c, 0, i-1);
+// //                 var s1 := input[i-1];
+                
+// //                 assert match c[i-1] case POZ(_) => isStringAValidNumber(s1);
+// //                 assert isStringAValidNumber(s1);
+                
+// //                 assert isInputCKT'(input, i);
+// //             }
+// //             case VARIABLE(X) => {
+// //                 assert isInputCKT'(input, i);
+// //             }
+// //     }
+// // }
+
+// lemma PozCellGivesValidNumber(c: circuit, pos: nat, input: seq<string>)
+//     requires isCircuitValid(c)
+//     requires pos < |c|
+//     requires isCircuitCellAPoz(c[pos])
+//     requires isCircuitGood(c)
+//     requires input == circuitToInput(c)
+//     requires |input| == |c|
+//     ensures isStringAValidNumber(input[pos])
+// {
+//     NthElementBridge(c, 0, pos);
+//     assert input[pos] == circuitCellToString(c[pos]);
+// }
 
 // lemma cktInputGivesValidCircuit(input:seq<string>)
 //     requires isInputCKT(input)
